\documentclass{article}
\usepackage{graphicx}
\graphicspath{ {/} }
\usepackage{setspace}
\doublespacing
\begin{document}

Consider the Fibonacci function, F(n) (see Proposition 3.20). Show by
induction that $F(n)4$ is $\Omega((3/2)n)$.\\\\

Lets find $c$ and $n_{0}$ such that $F(n) \geq c(\frac{3}{2})^{n}$\\
for $c = \frac{4}{9}$ and $n_{0} = 1$ everything works great\\
Inductive Hippotesis:\\
$F(k) \geq c(\frac{3}{2})^{k}$\\
\begin{math}
= F(k+1) + F(k-1)\\
\geq c(\frac{3}{2})^{k} + c(\frac{3}{2})^{k-1}\\
= c(\frac{3}{2})^{k-1}\cdot\frac{3}{2} + c(\frac{3}{2})^{k-1}\\
= c(\frac{3}{2})^{k-1}(\frac{3}{2}+1)\\
> c(\frac{3}{2})^{k-1}(\frac{3}{2})^{2}, \textnormal{ since } \frac{5}{2} > \frac{9}{4} \\
= c(\frac{3}{2})^{k+1}
\end{math}


\begin{center}
	\includegraphics[scale=0.3]{birb}
	http://www.simonfoucher.com/McGill/COMP250/Lectures/Math/lecture13.pdf
\end{center}

	
\end{document}


= F(k+1) + F(k-1)\\
\geq c(\frac{3}{2})^{k} + c(\frac{3}{2})^{k-1}\\
= c(\frac{3}{2})^{k-1}\cdot\frac{3}{2} + c(\frac{3}{2})^{k-1}\\
= c(\frac{3}{2})^{k-1}(\frac{3}{2}+1)\\
> c(\frac{3}{2})^{k-1}(1+1)\\
= c((\frac{3}{2})^{k-1}+ (\frac{3}{2})^{k-1})\\
= c((2\cdot (\frac{3}{2})^{k-1})\\
> c((\frac{3}{2}\cdot (\frac{3}{2})^{k-1})\\
= c(\frac{3}{2})^{k}\\

oohh god XD